Weidenbach_Book/CDCL_Conflict_Minimisation.thy
@@ -1,6 +1,6 @@
 theory CDCL_Conflict_Minimisation
   imports
-    Watched_Literals_Watch_List_Domain
+    Watched_Literals_Watch_List
     WB_More_Refinement
     WB_More_Refinement_List "List-Index.List_Index"
 begin
